Adapt S3/A2 to Imp_6_RefExample

src/Exercises/Imp_6_RefExample.v
@@ -1,1 +1,36 @@
-Require Import PPS.Exercises.Imp_5_Ref.
+Require Import PPS.Exercises.Imp_5_Ref PPS.Env EqNat Lists.List.
+Import ListNotations.
+
+Notation "E ; x" := (union E (cons x nil)) (at level 40).
+Notation "EM '|-R' e ⇓ v" := (evalR EM e v) (at level 80).
+
+Definition x := 0.
+Definition y := 1.
+Definition E : Env := [] ; (x, (42, Numeric Int)) ; (y, (32, Numeric Int)).
+Definition updTM := @updateTMap Ref Val beq_nat.
+Definition M : Memory := updTM (updTM (emptyTMap Null) 42 (VNum (VInt 2)))
+                               32 (VNum (VInt 5)).
+Definition exp : Exp := Op (Op (Num (VInt 3)) mult (Var (Numeric Int) y))
+                           plus
+                           (Var (Numeric Int) x).
+
+Example e : (E,M) |-R exp ⇓ (VNum (VInt 17)).
+Proof. eapply EvPlusR with (v1 := VInt 15) (v2 := VInt 2).
+       - eapply EvMultR with (v1 := VInt 3) (v2 := VInt 5).
+         + apply EvNumR.
+         + eapply EvVarR. apply LAxiom. reflexivity.
+         + apply EvTMult.
+           * apply EvTInt.
+           * eapply EvTVar. apply LAxiom.
+         + reflexivity.
+       - eapply EvVarR. apply LRule. apply LAxiom. reflexivity.
+       - apply EvTPlus.
+         + apply EvTMult.
+           * apply EvTInt.
+           * eapply EvTVar. apply LAxiom.
+         + eapply EvTVar. apply LRule. apply LAxiom.
+       - reflexivity.
+Qed.
+
+Example e2 : (E,M) |-R exp ⇓ (VNum (VInt 17)).
+Proof. repeat econstructor. Qed.
